\documentclass{article}
\usepackage[utf8]{inputenc}
\usepackage{amsfonts}
\usepackage{amsmath}
\usepackage{graphicx}
\usepackage[a4paper, total={6in, 8in}]{geometry}
\usepackage{setspace}
\usepackage{xcolor}

\everymath{\displaystyle}

\newcommand\tab[1][1cm]{\hspace*{#1}}
\doublespacing
\author{Frederic Becerril}

\newcommand{\important}[1]{{\color{red}\underline{\textbf{#1}}}}
\newcommand{\hbrace}[2]{\underset{#1}{\underbrace{#2}}}
\newcommand{\mylim}[2]{\underset{#1 \rightarrow #2}{\longrightarrow}}
\newcommand{\mysim}[2]{\underset{#1 \rightarrow #2}{\sim}}
% \newcommand{\citer}[2]{\og #2 \fg{} (#1)}
% \color{red}

\begin{document}

\part*{Exerice 6}

$X : \Omega \rightarrow \{0, \dots, N\}$ $N \geq 1$
\paragraph{\underline{Méthode 1}:} $\sum_{k = 0}^{N-1}P(X > k)$\\
$\tab = \sum_{k=0}^{N-1} \sum_{j = k+1}^N P(X=j)$ \vspace{2mm}\\
$\tab = \sum_{0 \leq k < j \leq N} P(X=j)$\\
$\tab = \sum_{j = 1}^N \sum_{k=0}^{j-1} P(X=j) = \sum_{j = 1}^N jP(X=j)$\\
\paragraph{\underline{Méthode 2}:\\}
$\sum_{k = 1}^N kP(X=k) = \sum_{k =1}^N k(P(X > k - 1) - P(X > k))$\\
$\tab[2.8cm] = \sum_{k =1}^N k\left(P(X > k - 1) - \sum_{k =1}^N P(X > k)\right)$\\
$\tab[2.8cm] = \sum_{k =0}^{N -1} (k + 1)P(X > k) - \sum_{k =1}^N kP(X > k)$\\
$\tab[2.8cm] = \sum_{k =0}^{N -1} (k + 1)P(X > k) -  \sum_{k = 0}^{N - 1} kP(X > k)$ (*)\\
$\tab[2.8cm] = \sum_{k =0}^{N -1} P(X > k)$\vspace{1cm}\\
(*) on a $\sum_{k =1}^N kP(X > k)$ = $\sum_{k = 0}^{N - 1} kP(X > k) - 0(P(X > 0)) + NP(X > N)$\\
or $P(X > N) = 0$ car $X$ ne peut pas être pas plus grand que N\\
Donc $\sum_{k =1}^N kP(X > k)$  = $\sum_{k = 0}^{N - 1} kP(X > k)$
\newpage
\noindent 1- $\Omega = \{1, \dots, N\}^n$\\
$Card(\Omega) = N^n$\\
$P(X \leq k) = \left(\frac{k}{N}\right)^n$\\
$P(X > k) = 1 - P(X \leq k) = 1 - \left(
    \frac{k}{N}
\right)^n$, $\forall k \geq 1$\\
$\sum_{k=0}^{N-1} P(X > k) = \sum_{k=0}^{N-1} \left(1 - \left(\frac{k}{N}\right)^n\right) = N - \sum_{k=1}^{N-1} \left(\frac{k}{N}\right)^n$\\
2- $P(X = k) = P(X \leq k) - P(X \leq k - 1) = \left(\frac{k}{N}\right)^n - \left(\frac{k-1}{N}\right)^n$, $\forall k \in \{1, \dots, N\}$
\end{document}