\documentclass{article}
\usepackage[utf8]{inputenc}
\usepackage{amsfonts}
\usepackage{amsmath}
\usepackage{graphicx}
\usepackage[a4paper, total={6in, 8in}]{geometry}
\usepackage{setspace}

\newcommand\tab[1][1cm]{\hspace*{#1}}
\onehalfspacing
\author{Frederic Becerril}

\begin{document}

\part*{Exerice 4}

$\bullet$ Soit $(E, <.|.>)$ un espace euclidien et $(x, y) \in E^2$\\
\begin{center}
    \begin{minipage}{0.75\textwidth}    
        \begin{itemize}
            \item[$<x + y | x + y>$] $= <x | x + y> + <y | x + y>$ (*)
            \item[] $=<x | x> + <x | y> + <y | x> + <y | y>$ (*)
            \item[] $=<x | x> + <x | y> + <x | y> + <y | y>$ (**) 
            \item[] $||x||^2 + ||y||^2 + 2 <x|y>$
        \end{itemize}
    \end{minipage}
\end{center}
(*) Bilinéarité du produit sclaire
(**) Symétrie du produit sclaire

\begin{center}
    \begin{minipage}{0.75\textwidth}    
        \begin{itemize}
            \item[$<x - y | x - y>$] $= <x | x - y> - <y | x - y>$
            \item[] $=<x | x> - <x | y> - (<y | x> - <y | y>)$
            \item[] $=<x | x> - <x | y> - <x | y> + <y | y>$ 
            \item[] $||x||^2 + ||y||^2 - 2 <x|y>$
        \end{itemize}
    \end{minipage}
\end{center}

\begin{center}
    \begin{minipage}{0.75\textwidth}    
        \begin{itemize}
            \item[$<x + y | x - y>$] $= <x | x - y> + <y | x - y>$
            \item[] $=<x | x> - <x | y> + <y | x> - <y | y>$
            \item[] $=<x | x> - <x | y> + <x | y> - <y | y>$
            \item[] $||x||^2 - ||y||^2$
        \end{itemize}
    \end{minipage}
\end{center}
$\bullet$ Soit $(x, y) \in E^2$
\begin{center}
    \begin{minipage}{0.75\textwidth}    
        \begin{itemize}
            \item[$||x + y||^2 + ||x - y||^2$] $= <x + y | x + y> +<x - y | x - y>$
            \item[] $= ||x||^2 + ||y||^2 + 2 <x|y> + ||x||^2 + ||y||^2 - 2 <x|y>$
            \item[] $= 2 * (||x||^2 + ||y||^2)$ 
        \end{itemize}
    \end{minipage}
\end{center}
$\bullet$ Soit $(x, y) \in E^2$
\begin{center}
    \begin{minipage}{0.75\textwidth}    
        \begin{itemize}
            \item[$2 + ||x + y||^2$] $= 2 + <x + y | x + y>$
            \item[] $=2 + ||x||^2 + ||y||^2 + 2 <x|y>$
            \item[] $\leq 2 + ||x||^2 + ||y||^2 + 2<x|y>$
            \item[] $= 2 * (1 + ||x||^2 + ||y||^2 + <x|y>)$
            \item[] $\leq 2 * (1 + ||x||^2 + ||y||^2 + ||x||^2||y||^2)$
            \item[] $=2 * (1 + ||x||^2) * (1 + ||y||^2)$  
        \end{itemize}
    \end{minipage}
\end{center}
\end{document}