\documentclass{article}
\usepackage[utf8]{inputenc}
\usepackage{amsfonts}
\usepackage{amsmath}
\usepackage{graphicx}
\usepackage[a4paper, total={6in, 8in}]{geometry}
\usepackage{setspace}

\everymath{\displaystyle}

\newcommand\tab[1][1cm]{\hspace*{#1}}
\doublespacing
\author{Frederic Becerril}

\NewDocumentCommand{\mylim}{ O{n} O{\infty}}{\underset{#1 \rightarrow #2}{\longrightarrow}}
\newcommand{\mysupp}[1]{\underset{x \in #1}{Sup}}
\newcommand{\mysim}[2]{\underset{#1 \rightarrow #2}{\sim}}
% \newcommand{\citer}[2]{\og #2 \fg{} (#1)}

\begin{document}

\part*{Exerice}

$\sum_{n \geq 0} \frac{n^2 - 10n + 1}{n!}x^n$\\
$a_n = \frac{n^2 - 10n + 1}{n!}$\\
Étudions $\frac{a_{n+1}}{a_n} = \frac{(n + 1)^2 - 10(n + 1) + 1}{(n + 1)!} * \frac{n!}{n^2 - 10n + 1}$\\
$\tab[2.42cm] = \frac{n^2 + 2n + 1 -10n -10 + 1}{n!(n+1)} * \frac{n!}{n^2 - 10n + 1}$\\
$\tab[2.42cm] = \frac{n^2 -8n -8}{(n + 1)(n^2 - 10n + 1)}$\\
$\tab[2.42cm] = \frac{n^2 -10n + 1}{(n + 1)(n^2 - 10n + 1)} + \frac{2n - 9}{(n + 1)(n^2 - 10n + 1)}$\\
$\tab[2.42cm] = \frac{1}{n + 1} + \frac{2(n + 1)}{(n + 1)(n^2 - 10n + 1)} - \frac{11}{(n + 1)(n^2 - 10n + 1)}$\\
$\tab[2.42cm] = \frac{1}{n + 1} + \frac{2}{(n^2 - 10n + 1)} - \frac{11}{(n + 1)(n^2 - 10n + 1)}$ or \\
$\tab[2.42cm] = \underset{\mylim 0}{\underbrace{\frac{1}{n + 1}}}
+ \underset{\mylim 0}{\underbrace{\frac{2}{(n^2 - 10n + 1)}}}
- \underset{\mylim 0}{\underbrace{\frac{11}{(n + 1)(n^2 - 10n + 1)}}}$\\
Donc $\frac{a_{n+1}}{a_n} \mylim 0$\\
Or d'après le critère d'Alembert on a R = $\frac{1}{0}$ qui par convention donne R = $\infty$ \\
On cherche une fonction tel que $f^{(n)}(0) = n^2 -10n + 1$\\
Soit S(x) = $\sum_{n \geq 0} \frac{n^2 - 10n + 1}{n!}x^n$\\
$n^2 -10n + 1$ = $n(n-1) + n - 10n + 1$ = $n(n -1) - 9n + 1$\\
$\frac{n^2 -10n + 1}{n!}$ = $\frac{n(n-1)}{n!} - 9\frac{n}{n!} + \frac{1}{n!}$\\
Pour $n \geq 2$\\
$\tab[2.25cm] = \frac{1}{(n-2)!} - 9\frac{1}{(n-1)!} + \frac{1}{n!}$\\
$a_0 = 1$\\
$a_1 = -8$\\
$\sum_{n \geq 0} \frac{n^2 - 10n + 1}{n!}x^n = 1 - 8x + \sum_{n \geq 2} (\frac{1}{(n-2)!} - 9\frac{1}{(n-1)!} + \frac{1}{n!})x^n$\\
$=1 - 8x + \sum_{n \geq 2} x^2 \frac{x^{n-2}}{(n-2)!} - 9\sum_{n \geq 2} x\frac{x^{n-1}}{(n-1)!} + \sum_{n \geq 2} \frac{x^n}{n!}$\\
$=1 - 8x + x^2\sum_{j \geq 0} \frac{x^{j}}{j!} - 9x\sum_{n \geq 1} x\frac{x^{k}}{k!} + \sum_{n \geq 2} \frac{x^n}{n!}$\\
$=1 - 8x + x^2\sum_{j \geq 0} \frac{x^{j}}{j!} - 9x(\sum_{n \geq 0} x\frac{x^{k}}{k!} -1) + \sum_{n \geq 0} \frac{x^n}{n!} -1 -x$\\
$=1 - 8x + x^2 e^x -9x (e^x -1) + e^x -1 -x$\\
$=(x^2 -9x + 1)e^x$\\

\end{document}